src/Parsers/Refinement/SharpenedExpressionPlusParenParseTree.v
@@ -11,7 +11,7 @@ Proof.
 Defined.
 
 Definition parser_informative (str : Coq.Strings.String.string)
-  : option (@simple_parse_of Ascii.ascii).
+  : option (@simple_parse_of_item Ascii.ascii).
 Proof.
   Time make_parser_informative ComputationalSplitter.
 Defined.
@@ -94,67 +94,109 @@ Proof.
   destruct_parses.
   exact n.
 Defined.
-(*
+
 Section evals.
-  Fixpoint evalT_productions {str ps} (pt : parse_of plus_expr_grammar str ps) : Type
-  with evalT_production {str p} (pt : parse_of_production plus_expr_grammar str p) : Type
-  with evalT_item {str it} (pt : parse_of_item plus_expr_grammar str it) : Type.
+  (* grammar_of_pregrammar
+  [[["expr" ::== "pexpr" || ("pexpr" "+") "expr";;
+  "pexpr" ::== "number" || ("(" "expr") ")";;
+  "number" ::== [0-9] || [0-9] "number"]]] *)
+  Fixpoint sevalT_productions (pt : @simple_parse_of Ascii.ascii) : Type
+  with sevalT_production (pt : @simple_parse_of_production Ascii.ascii) : Type
+  with sevalT_item (pt : @simple_parse_of_item Ascii.ascii) : Type.
   Proof.
-    { handle_evalT_parse. }
-    { handle_evalT_parse. }
-    { handle_evalT_parse.
-      { (* number case *)
-        exact nat. }
-      { (* pexpr case *)
-        exact nat. }
-      { (* expr case *)
-        exact nat. } }
+    { refine match pt with
+               | SimpleParseHead pt' => sevalT_production pt'
+               | SimpleParseTail pt' => sevalT_productions pt'
+             end. }
+    { refine match pt return Type with
+               | SimpleParseProductionNil => unit
+               | SimpleParseProductionCons p ps => (sevalT_item p * sevalT_production ps)%type
+             end. }
+    { refine match pt return Type with
+               | SimpleParseTerminal ch => unit (*{ ch' : _ | ch' = ch }*)
+               | SimpleParseNonTerminal _ _ => nat
+             end. }
   Defined.
 
-  (** Most of this is boilerplate.  It should be factored out, as it's
-      mostly common to all gramamrs (but there's some funky dependent
-      types stuff going on, which might be tricky to factor out. *)
-  Fixpoint eval_productions {str ps} (pt : parse_of plus_expr_grammar str ps) : evalT_productions pt
-  with eval_production {str p} (pt : parse_of_production plus_expr_grammar str p) : evalT_production pt
-  with eval_item {str it} (pt : parse_of_item plus_expr_grammar str it) : evalT_item pt.
+  Definition impossible {T} : T -> nat.
   Proof.
-    { handle_eval_parse. }
-    { handle_eval_parse. }
-    { handle_eval_parse;
-      (** Here's the grammar-specific part, which handles each type of production *)
-      try match type of eval_production with
-          | ({ ch' : ascii | ch' = ?ch } * unit)%type (* [0-9] *)
-            => match goal with
-               | [ Hcheck : is_true (?P ch), Hp : ?P = (fun ch0 => (Compare_dec.leb 48 (?f ch0) && Compare_dec.leb (?f ch0) 57)%bool) |- _ ]
-                 => exact (f (proj1_sig (fst eval_production)) - 48 (* "0" *))
-               end
-          | (nat * unit)%type
-            => match goal with
-               | [ Hcheck : context["number" = "number"] |- _ ] (* "number" *)
-                 => exact (fst eval_production)
-               | [ Hcheck : context["pexpr" = "pexpr"] |- _ ] (* "pexpr" *)
-                 => exact (fst eval_production)
-               end
-          end;
-      try match type of eval_productions with
-          | ({ ch' : ascii | ch' = ?ch } * (nat * unit))%type (* [0-9] "number" *)
-            => match goal with
-               | [ Hcheck : is_true (?P ch), Hp : ?P = (fun ch0 => (Compare_dec.leb 48 (?f ch0) && Compare_dec.leb (?f ch0) 57)%bool) |- _ ]
-                 => exact (10 * (f (proj1_sig (fst eval_productions)) - 48 (* "0" *))
-                           + fst (snd eval_productions))
-               end
-          | ({ch1 : ascii | ch1 = ?l} * (nat * ({ch2 : ascii | ch2 = ?r} * ())))%type (* "(" "expr" ")" *)
-            => match goal with
-               | [ Hcheckl : is_true (?Pl l), Hcheckr : is_true (?Pr r),
-                                                        Hl : ?Pl = Equality.ascii_beq "("%char, Hr : ?Pr = Equality.ascii_beq ")"%char |- _ ]
-                 => exact (fst (snd eval_productions))
-               end
-          | (nat * ({ch1 : ascii | ch1 = ?ch} * (nat * ())))%type (* "pexpr" "+" "expr" *)
-            => match goal with
-               | [ Hcheck : is_true (?P ch), HP : ?P = Equality.ascii_beq "+"%char |- _ ]
-                 => exact (fst eval_productions + fst (snd (snd eval_productions)))
-               end
-          end. }
+    intro; exact 0.
+  Qed.
+
+  Fixpoint seval_productions (pt : @simple_parse_of Ascii.ascii) : sevalT_productions pt
+  with seval_production (pt : @simple_parse_of_production Ascii.ascii) : sevalT_production pt
+  with seval_item (pt : @simple_parse_of_item Ascii.ascii) : sevalT_item pt.
+  Proof.
+    { destruct pt; simpl; eauto with nocore. }
+    { destruct pt; simpl; eauto using tt, pair with nocore. }
+    { destruct pt as [ch|nt pt]; simpl.
+      { eexists; reflexivity. }
+      { specialize (seval_productions pt).
+        revert seval_productions.
+        destruct (string_dec nt "number");
+          [
+          | destruct (string_dec nt "pexpr");
+            [
+            | destruct (string_dec nt "expr");
+              [
+              | exact impossible ] ] ].
+        { (* "number" ::== [0-9] || [0-9] "number"]]] *)
+          refine match pt return sevalT_productions pt -> nat with
+                   | SimpleParseHead
+                       (SimpleParseTerminal ch::[])
+                     (* [0-9] *)
+                     => fun _ => opt.nat_of_ascii ch - 48 (* opt.nat_of_ascii "0" is 48 *)
+                   | SimpleParseTail
+                       (SimpleParseHead
+                          (SimpleParseTerminal ch::SimpleParseNonTerminal number pt'::[]))
+                     (* [0-9] "number" *)
+                     => fun v
+                        => ((opt.nat_of_ascii ch - 48 (* opt.nat_of_ascii "0" is 48 *))
+                            * 10
+                            + fst (snd v))%nat
+                   | _ => impossible
+                 end. }
+        { (* "pexpr" ::== "number" || "(" "expr" ")";; *)
+          refine match pt return sevalT_productions pt -> nat with
+                   | SimpleParseHead
+                       (SimpleParseNonTerminal number pt'::[])
+                     (* "number" *)
+                     => fst
+                   | SimpleParseTail
+                       (SimpleParseHead
+                          (SimpleParseTerminal ch::SimpleParseNonTerminal expr pt'::SimpleParseTerminal ch'::[]))
+                     (* "(" "expr" ")" *)
+                     => fun v => fst (snd v)
+                   | _ => impossible
+                 end. }
+        { (* "expr" ::== "pexpr" || "pexpr" "+" "expr" *)
+          refine match pt return sevalT_productions pt -> nat with
+                   | SimpleParseHead
+                       (SimpleParseNonTerminal pexpr pt'::[])
+                     (* "pexpr" *)
+                     => fst
+                   | SimpleParseTail
+                       (SimpleParseHead
+                          (SimpleParseNonTerminal pexpr n1::SimpleParseTerminal plus::SimpleParseNonTerminal expr n2::[]))
+                     (* "pexpr" "+" "expr" *)
+                     => fun v => fst v + fst (snd (snd v))
+                   | _ => impossible
+                 end. } } }
   Defined.
-End eval.
-*)
+End evals.
+
+Definition parser_eval (str : Coq.Strings.String.string)
+  : option nat.
+Proof.
+  refine match parser_informative str with
+         | Some (SimpleParseNonTerminal nt pt)
+           => let n := seval_item (SimpleParseNonTerminal nt pt) in
+              Some n
+         | Some (SimpleParseTerminal _) => None
+         | None => None
+         end.
+Defined.
+
+Check let n := 3 in eq_refl (Some n) <: parser_eval "(1+1)+1" = Some n.
+Check let n := 5 in eq_refl (Some n) <: parser_eval "((1+1)+(1+1))+1" = Some n.
+Check let n := 55 in eq_refl (Some n) <: parser_eval "(((((55)))))" = Some n.
