src/Parsers/ParserInterface.v
@@ -73,7 +73,7 @@ Record Parser {Char} (G : grammar Char)
                            parse_of_item G str (NonTerminal (Start_symbol G))
                            -> has_parse str = true;
 
-    parse : @String Char HSLM -> option (@simple_parse_of Char);
+    parse : @String Char HSLM -> option (@simple_parse_of_item Char);
     (** find the parse tree of the string as the start symbol of the grammar *)
 
     parse_correct : forall str, has_parse str = if parse str then true else false
