src/Parsers/Refinement/SharpenedABStarParseTree.v
@@ -24,7 +24,7 @@ Proof.
 Abort.
 
 Definition ab_star_parser_informative (str : Coq.Strings.String.string)
-  : option (@simple_parse_of Ascii.ascii).
+  : option (@simple_parse_of_item Ascii.ascii).
 Proof.
   Time make_parser_informative (@ComputationalSplitter _ String.string_stringlike _ _). (* 0.124 s *)
 Defined.
